src/Proofs/Transfer.v
@@ -3,11 +3,11 @@ Require Import UrsusEnvironment.Solidity.current.LocalGenerator.
 Require Import FinProof.Lib.HMapList.
 
 Require Import UMLang.ExecGenerator.
+Require Import Common.
 
 Require Import EIP20.
 Import EIP20.
 
-Require Import Common.
 Require Import EvalExecs.Transfer.
 
 
@@ -320,6 +320,491 @@ Proof.
     end.
 Qed.
 
+
+Lemma transfer_others_balances: forall (_to :  address) 
+                            (_value : uint256)
+                            (l: LedgerLRecord rec), 
+    let l0 := {$$ l with Ledger_LocalState := default $$} in
+    let l' := exec_state (Uinterpreter (@transfer rec def _ _ _ _ _to _value)) l0 in
+    let msg_sender := VMState_ι_msg_sender (l.(Ledger_VMState)) in
+    let balances0 := (_balances (l.(Ledger_MainState))) in
+    _to <> msg_sender -> 
+    _balances (l'.(Ledger_MainState)) = 
+    if (xIntGeb (balances0 [msg_sender])  _value : bool) then 
+        (balances0 [msg_sender] ← (xIntMinus (balances0 [msg_sender]) _value)) [_to] ← 
+            (xIntPlus (balances0 [_to]) _value) else balances0.
+Proof. 
+    intros. transfer_start l l0 l'.
+    compute_rhs.    
+    compute in balances0, msg_sender.
+
+    match goal with
+    | |- context [if ?b then false else true] => remember b
+    end.    
+    
+    case_eq b; intros; auto.
+    remember (eqb _to v4).
+    destruct y.
+    - symmetry in Heqy. 
+      rewrite BoolEq.eqb_spec_intro in Heqy.
+      subst msg_sender. contradiction.
+    - 
+
+    remember (s0 [_to] ?).
+    destruct y.
+
+    +
+
+    erewrite 2lookup_some_find with (k:=_to).
+    3: unshelve erewrite lookup_addAdjust_another.    
+    3: refine (BoolEq.pair_eqb_spec (X:=Z) (Y:=XUBInteger 256)).
+    2, 3: setoid_rewrite <- Heqy0.
+    2, 3: reflexivity.
+    2: assumption.
+    auto.
+
+    +
+    erewrite 2lookup_none_find with (k:=_to).
+    3: unshelve erewrite lookup_addAdjust_another.    
+    3: refine (BoolEq.pair_eqb_spec (X:=Z) (Y:=XUBInteger 256)).
+    2, 3: auto.
+    2: assumption.
+    auto.
+Qed.    
+
+Lemma transfer_msg_sender_member_balances: forall (_to :  address) 
+                            (_value : uint256)
+                            (l: LedgerLRecord rec), 
+    let l0 := {$$ l with Ledger_LocalState := default $$} in
+    let l' := exec_state (Uinterpreter (@transfer rec def _ _ _ _ _to _value)) l0 in
+    let msg_sender := VMState_ι_msg_sender (l.(Ledger_VMState)) in
+    let balances0 := (_balances (l.(Ledger_MainState))) in     
+    _to = msg_sender -> 
+    keysDistinct balances0 ->
+    hmapIsMember (H7 := @pair_xbool_equable bool _ Z _ uint256 _  ) msg_sender balances0  = true ->
+    _balances (l'.(Ledger_MainState)) = balances0.
+Proof.
+    intros. transfer_start l l0 l'.
+    compute_rhs.    
+    compute in balances0, msg_sender.
+
+    match goal with
+    | |- context [if ?b then false else true] => remember b
+    end.    
+    
+    case_eq b; intros; auto.
+    subst msg_sender.
+    subst v4.
+
+    apply member_true_lookup in H1.
+    destruct H1.    
+
+    erewrite 2lookup_some_find with (k:=_to).
+    3: erewrite lookup_some_find with (k:=_to).    
+    3: unshelve erewrite lookup_addAdjust.    
+    3: refine (BoolEq.pair_eqb_spec (X:=Z) (Y:=XUBInteger 256)).
+    3: reflexivity.        
+    2,3: setoid_rewrite H.    
+    2,3: reflexivity.
+
+    erewrite insert_insert.
+    unfold xHMapInsert. simpl.
+    match goal with
+    | |- context [@addAdjustListPair _ _ _ ?a ?v _] => remember v
+    end.
+    enough (x0 = x).
+    destruct s0.
+    erewrite member_addAdjust; auto.
+    rewrite H1. auto.
+    subst x0.
+    destruct x, _value. simpl.
+    f_equal.
+    erewrite lookup_some_find with (k:=_to) in Heqb.
+    2: setoid_rewrite H.
+    2: reflexivity.
+    simpl in Heqb.
+    rewrite H2 in Heqb.
+    symmetry in Heqb.
+    apply N.leb_le in Heqb.
+    lia.
+    Unshelve.
+    all: refine (BoolEq.pair_eqb_spec (X:=Z) (Y:=XUBInteger 256)).
+Qed.    
+
+Lemma transfer_msg_sender_not_member_balances: forall (_to :  address) 
+                            (_value : uint256)
+                            (l: LedgerLRecord rec), 
+    let l0 := {$$ l with Ledger_LocalState := default $$} in
+    let l' := exec_state (Uinterpreter (@transfer rec def _ _ _ _ _to _value)) l0 in
+    let msg_sender := VMState_ι_msg_sender (l.(Ledger_VMState)) in
+    let balances0 := (_balances (l.(Ledger_MainState))) in     
+    _to = msg_sender -> 
+    keysDistinct balances0 ->
+    hmapIsMember (H7 := @pair_xbool_equable bool _ Z _ uint256 _  ) msg_sender balances0  = false ->
+    _balances (l'.(Ledger_MainState)) =
+    if (xIntGeb (balances0 [msg_sender])  _value : bool) then 
+         balances0 [msg_sender] ← default
+    else balances0.
+Proof.
+    intros. transfer_start l l0 l'.
+    compute_rhs.    
+    compute in balances0, msg_sender.
+
+    match goal with
+    | |- context [if ?b then false else true] => remember b
+    end.    
+    
+    case_eq b; intros; auto.
+    subst msg_sender.
+    subst v4.
+
+    apply member_false_lookup in H1.    
+
+    erewrite lookup_some_find with (k:=_to).
+    erewrite lookup_none_find with (k:=_to).    
+    3: erewrite lookup_none_find with (k:=_to).    
+    3: unshelve erewrite lookup_addAdjust.    
+    3: refine (BoolEq.pair_eqb_spec (X:=Z) (Y:=XUBInteger 256)).
+    2, 3, 4: auto.
+    enough (_value = default).
+    subst _value.
+    simpl.
+    erewrite insert_insert.        
+    simpl.
+    match goal with
+    | |- context [@addAdjustListPair _ _ _ ?a ?v _] => remember v
+    end.
+    enough (x = default).
+    rewrite H. auto.
+    subst x.
+    simpl default.
+    f_equal.
+
+
+    simpl in Heqb.
+    rewrite H2 in Heqb.
+    symmetry in Heqb.
+    apply N.leb_le in Heqb.
+    destruct _value.
+    simpl default.
+    f_equal.
+    erewrite lookup_none_find with (k:=_to) in Heqb.
+    simpl in Heqb.    
+    (* compute in Heqb. *)
+    vm_compute.
+    lia.
+    subst balances0.
+    auto.
+    Unshelve.
+    refine (BoolEq.pair_eqb_spec (X:=Z) (Y:=XUBInteger 256)).
+Qed.
+
+Lemma transfer_balances_keysDistinct: forall (_to :  address) 
+                            (_value : uint256)
+                            (l: LedgerLRecord rec), 
+    let l0 := {$$ l with Ledger_LocalState := default $$} in
+    let l' := exec_state (Uinterpreter (@transfer rec def _ _ _ _ _to _value)) l0 in
+    let msg_sender := VMState_ι_msg_sender (l.(Ledger_VMState)) in
+    let balances0 := (_balances (l.(Ledger_MainState))) in
+    let balances := (_balances (l'.(Ledger_MainState))) in     
+    keysDistinct balances0 ->  keysDistinct balances.
+Proof.
+    intros.
+    remember (xIntGeb (balances0 [msg_sender])  _value : bool) as b1.
+    remember (eqb _to msg_sender) as b2.
+    remember (hmapIsMember (H7 := @pair_xbool_equable bool _ Z _ uint256 _  ) msg_sender balances0) as b3.
+    subst balances. subst l'. subst l0. subst balances0. subst msg_sender.
+    destruct b1, b2, b3. 
+    -   rewrite transfer_msg_sender_member_balances; auto.  
+        apply BoolEq.eqb_spec_intro. auto.
+    -   rewrite transfer_msg_sender_not_member_balances; auto.
+        setoid_rewrite <- Heqb1.
+        apply insert_kd. assumption.
+        apply BoolEq.eqb_spec_intro. auto.
+    -   rewrite transfer_others_balances; auto.
+        rewrite <- Heqb1.
+        repeat apply insert_kd. assumption.
+        unfold not; intros. apply BoolEq.eqb_spec_intro in H0.
+        rewrite H0 in Heqb2. discriminate.
+    -   rewrite transfer_others_balances; auto.
+        rewrite <- Heqb1.
+        repeat apply insert_kd. assumption.
+        unfold not; intros. apply BoolEq.eqb_spec_intro in H0.
+        rewrite H0 in Heqb2. discriminate.
+    -   rewrite transfer_msg_sender_member_balances; auto.
+        apply BoolEq.eqb_spec_intro. auto.
+    -   rewrite transfer_msg_sender_not_member_balances; auto.
+        rewrite <- Heqb1. assumption.
+        apply BoolEq.eqb_spec_intro. auto.
+    -   rewrite transfer_others_balances; auto.
+        rewrite <- Heqb1. assumption.
+        unfold not; intros. apply BoolEq.eqb_spec_intro in H0.
+        rewrite H0 in Heqb2. discriminate.
+    -   rewrite transfer_others_balances; auto.
+        rewrite <- Heqb1. assumption.
+        unfold not; intros. apply BoolEq.eqb_spec_intro in H0.
+        rewrite H0 in Heqb2. discriminate.
+Qed.
+
+
+
+
+
+Lemma transfer_balances_sum: forall (_to :  address) 
+                            (_value : uint256)
+                            (l: LedgerLRecord rec), 
+    let l0 := {$$ l with Ledger_LocalState := default $$} in
+    let l' := exec_state (Uinterpreter (@transfer rec def _ _ _ _ _to _value)) l0 in
+    let msg_sender := VMState_ι_msg_sender (l.(Ledger_VMState)) in
+    let balances0 := (_balances (l.(Ledger_MainState))) in
+    let balances := (_balances (l'.(Ledger_MainState))) in     
+    keysDistinct balances0 ->    
+    hmapBSum balances = hmapBSum balances0.
+Proof.
+    intros.
+    remember (xIntGeb (balances0 [msg_sender])  _value : bool) as b1.
+    remember (eqb _to msg_sender) as b2.
+    remember (hmapIsMember (H7 := @pair_xbool_equable bool _ Z _ uint256 _  ) msg_sender balances0) as b3.
+    subst balances. subst l'. subst l0. subst balances0. subst msg_sender.
+    destruct b1, b2, b3.
+    - (* 1/8 *) rewrite transfer_msg_sender_member_balances; auto.
+      apply BoolEq.eqb_spec_intro. auto.
+    - (* 2/8 *) rewrite transfer_msg_sender_not_member_balances; auto.
+      setoid_rewrite <- Heqb1.
+      unfold hmapBSum.
+      rewrite mapBN2N_addAdjust.
+      rewrite hmapSumAdjust.
+      rewrite lookup_none_find.
+      simpl. f_equal. unfold N.zero. remember (hmapSum (mapBN2N (_balances (Ledger_MainState l)))).
+      setoid_rewrite <- Heqn. lia.
+      symmetry in Heqb3.
+      apply member_false_lookup in Heqb3. 
+      rewrite mapBN2N_hmapLookup2.
+      setoid_rewrite Heqb3. auto.
+      1,4: refine pair_xbool_equable.    
+      1,3: refine BoolEq.pair_eqb_spec.
+      2: assumption.
+      apply mapBN2N_keysDistinct. assumption.
+      apply BoolEq.eqb_spec_intro.
+      auto.
+    - (* 3/8 *) rewrite transfer_others_balances; auto.
+       rewrite <- Heqb1.
+       unfold hmapBSum.
+       repeat rewrite mapBN2N_addAdjust.
+       repeat rewrite hmapSumAdjust.
+       remember (hmapSum (mapBN2N (_balances (Ledger_MainState l)))).
+       setoid_rewrite <- Heqn.
+       remember ((mapBN2N (_balances (Ledger_MainState l))) [_to]?).
+       destruct y.
+       + erewrite 2lookup_some_find with (k:=_to).
+         2: erewrite lookup_addAdjust_another.
+         3: unfold not.
+         3: intros.         
+         3: apply BoolEq.eqb_spec_intro in H0.
+         3: rewrite H0 in Heqb2.
+         3: discriminate.
+         2: setoid_rewrite <- Heqy.
+         2: reflexivity.
+         rewrite mapBN2N_hmapLookup2 in Heqy.
+         all: cycle 3.
+         enough ((_balances (Ledger_MainState l)) [_to] ? = Some (Build_XUBInteger n0)).
+         setoid_rewrite H0. reflexivity.
+         rewrite mapBN2N_hmapLookup2 in Heqy.         
+         remember ((_balances (Ledger_MainState l)) [_to] ?).
+         setoid_rewrite <- Heqy0 in Heqy.         
+         destruct y. simpl in Heqy. inversion Heqy.
+         destruct x.  auto. inversion Heqy.
+         all: cycle 2.         
+
+         rewrite mapBN2N_hmapLookup.   
+         remember ((_balances (Ledger_MainState l))
+         [VMState_ι_msg_sender (Ledger_VMState l)]).
+         setoid_rewrite <- Heqx.
+         destruct x, _value.
+         simpl. 
+         f_equal.
+         enough(n1 >= n2).
+         enough(n >= n1). lia.
+         2: symmetry in Heqb1.
+         2: apply N.leb_le in Heqb1.
+         2: lia. 
+         subst n. 
+         enough (n1 = ((mapBN2N (_balances (Ledger_MainState l))) [VMState_ι_msg_sender (Ledger_VMState l)])).
+         subst n1.
+         apply hmapSumGE.
+         rewrite mapBN2N_hmapLookup.
+         setoid_rewrite <- Heqx.
+         auto.
+         1,3,5,7: refine pair_xbool_equable.    
+         1,2,3,4: refine BoolEq.pair_eqb_spec.
+         +
+         erewrite 2lookup_none_find with (k:=_to).
+         2: erewrite lookup_addAdjust_another.
+         3: unfold not.
+         3: intros.         
+         3: apply BoolEq.eqb_spec_intro in H0.
+         3: rewrite H0 in Heqb2.
+         3: discriminate.
+         2: setoid_rewrite <- Heqy.
+         2: reflexivity.
+         rewrite mapBN2N_hmapLookup.   
+         remember ((_balances (Ledger_MainState l))
+         [VMState_ι_msg_sender (Ledger_VMState l)]).
+         setoid_rewrite <- Heqx.
+         destruct x, _value.
+         simpl. 
+         f_equal.
+         unfold N.zero.
+         enough(n0 >= n1).
+         enough(n >= n0). lia.
+         2: symmetry in Heqb1.
+         2: apply N.leb_le in Heqb1.
+         2: lia. 
+         subst n. 
+         enough (n0 = ((mapBN2N (_balances (Ledger_MainState l))) [VMState_ι_msg_sender (Ledger_VMState l)])).
+         subst n0.
+         apply hmapSumGE.
+         rewrite mapBN2N_hmapLookup.
+         setoid_rewrite <- Heqx.
+         auto.
+         1,3: refine pair_xbool_equable.    
+         1,2: refine BoolEq.pair_eqb_spec.
+         rewrite mapBN2N_hmapLookup2 in Heqy.
+         remember ((_balances (Ledger_MainState l)) [_to] ?).         
+         setoid_rewrite <- Heqy0.
+         destruct y.
+         setoid_rewrite <- Heqy0 in Heqy.
+         inversion Heqy.
+         auto.
+         refine pair_xbool_equable.
+         refine BoolEq.pair_eqb_spec.
+         + apply mapBN2N_keysDistinct. assumption.
+         + apply insert_kd. apply mapBN2N_keysDistinct. assumption.
+         + refine pair_xbool_equable.
+         + refine BoolEq.pair_eqb_spec.
+         + assumption.
+         + refine pair_xbool_equable.
+         + refine BoolEq.pair_eqb_spec.
+         + apply insert_kd. assumption.
+         + unfold not; intros. apply BoolEq.eqb_spec_intro in H0.
+           rewrite H0 in Heqb2. discriminate.
+    - (* 4/8 *) rewrite transfer_others_balances; auto.
+       rewrite <- Heqb1.
+       unfold hmapBSum.
+       repeat rewrite mapBN2N_addAdjust.
+       repeat rewrite hmapSumAdjust.
+       remember (hmapSum (mapBN2N (_balances (Ledger_MainState l)))).
+       setoid_rewrite <- Heqn.
+       remember ((mapBN2N (_balances (Ledger_MainState l))) [_to]?).
+       destruct y.
+       + erewrite 2lookup_some_find with (k:=_to).
+         2: erewrite lookup_addAdjust_another.
+         3: unfold not.
+         3: intros.         
+         3: apply BoolEq.eqb_spec_intro in H0.
+         3: rewrite H0 in Heqb2.
+         3: discriminate.
+         2: setoid_rewrite <- Heqy.
+         2: reflexivity.
+         rewrite mapBN2N_hmapLookup2 in Heqy.
+         all: cycle 3.
+         enough ((_balances (Ledger_MainState l)) [_to] ? = Some (Build_XUBInteger n0)).
+         setoid_rewrite H0. reflexivity.
+         rewrite mapBN2N_hmapLookup2 in Heqy.         
+         remember ((_balances (Ledger_MainState l)) [_to] ?).
+         setoid_rewrite <- Heqy0 in Heqy.         
+         destruct y. simpl in Heqy. inversion Heqy.
+         destruct x.  auto. inversion Heqy.
+         all: cycle 2.         
+
+         rewrite mapBN2N_hmapLookup.   
+         remember ((_balances (Ledger_MainState l))
+         [VMState_ι_msg_sender (Ledger_VMState l)]).
+         setoid_rewrite <- Heqx.
+         destruct x, _value.
+         simpl. 
+         f_equal.
+         enough(n1 >= n2).
+         enough(n >= n1). lia.
+         2: symmetry in Heqb1.
+         2: apply N.leb_le in Heqb1.
+         2: lia. 
+         subst n. 
+         enough (n1 = ((mapBN2N (_balances (Ledger_MainState l))) [VMState_ι_msg_sender (Ledger_VMState l)])).
+         subst n1.
+         apply hmapSumGE.
+         rewrite mapBN2N_hmapLookup.
+         setoid_rewrite <- Heqx.
+         auto.
+         1,3,5,7: refine pair_xbool_equable.    
+         1,2,3,4: refine BoolEq.pair_eqb_spec.
+         +
+         erewrite 2lookup_none_find with (k:=_to).
+         2: erewrite lookup_addAdjust_another.
+         3: unfold not.
+         3: intros.         
+         3: apply BoolEq.eqb_spec_intro in H0.
+         3: rewrite H0 in Heqb2.
+         3: discriminate.
+         2: setoid_rewrite <- Heqy.
+         2: reflexivity.      
+
+         rewrite mapBN2N_hmapLookup.   
+         remember ((_balances (Ledger_MainState l))
+         [VMState_ι_msg_sender (Ledger_VMState l)]).
+         setoid_rewrite <- Heqx.
+         destruct x, _value.
+         simpl. 
+         f_equal.
+         unfold N.zero.
+         enough(n0 >= n1).
+         enough(n >= n0). lia.
+         2: symmetry in Heqb1.
+         2: apply N.leb_le in Heqb1.
+         2: lia. 
+         subst n. 
+         enough (n0 = ((mapBN2N (_balances (Ledger_MainState l))) [VMState_ι_msg_sender (Ledger_VMState l)])).
+         subst n0.
+         apply hmapSumGE.
+         rewrite mapBN2N_hmapLookup.
+         setoid_rewrite <- Heqx.
+         auto.
+         1,3: refine pair_xbool_equable.    
+         1,2: refine BoolEq.pair_eqb_spec.
+         rewrite mapBN2N_hmapLookup2 in Heqy.
+         remember ((_balances (Ledger_MainState l)) [_to] ?).         
+         setoid_rewrite <- Heqy0.
+         destruct y.
+         setoid_rewrite <- Heqy0 in Heqy.
+         inversion Heqy.
+         auto.
+         refine pair_xbool_equable.
+         refine BoolEq.pair_eqb_spec.
+         + apply mapBN2N_keysDistinct. assumption.
+         + apply insert_kd. apply mapBN2N_keysDistinct. assumption.
+         + refine pair_xbool_equable.
+         + refine BoolEq.pair_eqb_spec.
+         + assumption.
+         + refine pair_xbool_equable.
+         + refine BoolEq.pair_eqb_spec.
+         + apply insert_kd. assumption.
+         + unfold not; intros. apply BoolEq.eqb_spec_intro in H0.
+           rewrite H0 in Heqb2. discriminate.  
+      - (* 5/8 *) rewrite transfer_msg_sender_member_balances; auto.
+        apply BoolEq.eqb_spec_intro. auto.
+      - (* 6/8 *) rewrite transfer_msg_sender_not_member_balances; auto.
+        rewrite <- Heqb1. auto.
+        apply BoolEq.eqb_spec_intro. auto.
+      - (* 7/8 *) rewrite transfer_others_balances; auto.
+        rewrite <- Heqb1. auto.
+        unfold not; intros. apply BoolEq.eqb_spec_intro in H0.
+        rewrite H0 in Heqb2. discriminate.
+      - (* 8/8 *) rewrite transfer_others_balances; auto.
+        rewrite <- Heqb1. auto.
+        unfold not; intros. apply BoolEq.eqb_spec_intro in H0.
+        rewrite H0 in Heqb2. discriminate.
+Qed.        
+          
 
 Lemma transfer_allowed_unchanged: forall (_to :  address) 
                             (_value : uint256)
