src/Proofs/TransferFrom.v
@@ -3,11 +3,11 @@ Require Import UrsusEnvironment.Solidity.current.LocalGenerator.
 Require Import FinProof.Lib.HMapList.
 
 Require Import UMLang.ExecGenerator.
+Require Import Common.
 
 Require Import EIP20.
 Import EIP20.
 
-Require Import Common.
 Require Import EvalExecs.TransferFrom.
 
 Opaque Common.hmapFindWithDefault
@@ -462,3 +462,555 @@ Proof.
       auto.
       assumption.
 Qed. 
+
+Lemma transferFrom_others_balances: forall (_from :  address) (_to :  address) 
+                            (_value : uint256)
+                            (l: LedgerLRecord rec), 
+    let l0 := {$$ l with Ledger_LocalState := default $$} in
+    let l' := exec_state (Uinterpreter (@transferFrom rec def _ _ _ _ _from _to _value)) l0 in
+    let msg_sender := VMState_ι_msg_sender (l.(Ledger_VMState)) in
+    let balances0 := (_balances (l.(Ledger_MainState))) in
+    let allowed0 := (_allowed (l.(Ledger_MainState))) in
+    _from <> _to  -> 
+    _balances (l'.(Ledger_MainState)) = 
+    if ((xIntGeb balances0 [_from]  _value : bool) && 
+        (xIntGeb allowed0 [_from] [msg_sender] _value : bool) ) then 
+        (balances0 [_to] ← (xIntPlus (balances0 [_to]) _value)) 
+          [_from] ← (xIntMinus (balances0 [_from]) _value) else balances0.
+Proof. 
+    intros. transferFrom_start l l0 l'.
+    compute_rhs.    
+    compute in balances0, allowed0, msg_sender.
+
+    match goal with
+    | |- context [if ?b then false else true] => remember b
+    end.    
+    
+    case_eq b; intros; auto.
+
+    match goal with
+    | |- context [if ?b then _ else _] => remember b
+    end.    
+    
+    destruct b0.
+    - remember (s0[_from]?).
+      destruct y.
+      + erewrite lookup_some_find.
+        2: erewrite lookup_addAdjust_another; auto.
+        2: setoid_rewrite <- Heqy.
+        2: reflexivity.
+        erewrite lookup_some_find with (k:=_from).
+        2: setoid_rewrite <- Heqy.
+        2: reflexivity.
+        auto.
+      + erewrite lookup_none_find with (k:=_from).
+        2: erewrite lookup_addAdjust_another; auto.
+        erewrite lookup_none_find with (k:=_from).
+        auto. auto.
+    - remember (s0[_from]?).
+      destruct y.
+      + erewrite lookup_some_find.
+        2: erewrite lookup_addAdjust_another; auto.
+        2: setoid_rewrite <- Heqy.
+        2: reflexivity.
+        erewrite lookup_some_find with (k:=_from).
+        2: setoid_rewrite <- Heqy.
+        2: reflexivity.
+        auto.
+      + erewrite lookup_none_find with (k:=_from).
+        2: erewrite lookup_addAdjust_another; auto.
+        erewrite lookup_none_find with (k:=_from).
+        auto. auto.   
+    Unshelve.
+    all: refine (BoolEq.pair_eqb_spec (X:=Z) (Y:=XUBInteger 256)).     
+Qed.
+
+
+Lemma transferFrom_from_member_balances: forall (_from :  address) (_to :  address) 
+                            (_value : uint256)
+                            (l: LedgerLRecord rec), 
+    let l0 := {$$ l with Ledger_LocalState := default $$} in
+    let l' := exec_state (Uinterpreter (@transferFrom rec def _ _ _ _ _from _to _value)) l0 in
+    let msg_sender := VMState_ι_msg_sender (l.(Ledger_VMState)) in
+    let balances0 := (_balances (l.(Ledger_MainState))) in     
+    _from = _to -> 
+    keysDistinct balances0 ->
+    hmapIsMember (H7 := @pair_xbool_equable bool _ Z _ uint256 _  ) _from balances0  = true ->
+    _balances (l'.(Ledger_MainState)) = balances0.
+Proof.
+    intros. transferFrom_start l l0 l'.
+    compute_rhs.    
+    compute in balances0, msg_sender.
+
+    match goal with
+    | |- context [if ?b then false else true] => remember b
+    end.    
+    
+    case_eq b; intros; auto.
+
+    match goal with
+    | |- context [if ?b then _ else _] => remember b
+    end.    
+    
+    rewrite H.
+    destruct b0.
+
+    - remember (s0[_to]?).
+      destruct y.
+      + erewrite lookup_some_find.
+        2: erewrite lookup_addAdjust; auto.        
+        erewrite lookup_some_find with (k:=_to).
+        2: setoid_rewrite <- Heqy.
+        2: reflexivity.
+        erewrite insert_insert.
+        unfold xHMapInsert. simpl.
+        match goal with
+        | |- context [@addAdjustListPair _ _ _ ?a ?v _] => remember v
+        end.
+        enough (x0 = x).
+        destruct s0.
+        erewrite member_addAdjust; auto.
+        rewrite H3. auto.
+        subst x0.
+        destruct x, _value. simpl.
+        f_equal. lia.
+      + subst _from.
+        apply member_true_lookup in H1.
+        destruct H1.
+        setoid_rewrite H in Heqy.
+        discriminate.
+    - remember (s0[_to]?).
+      destruct y.
+      + erewrite lookup_some_find.
+        2: erewrite lookup_addAdjust; auto.        
+        erewrite lookup_some_find with (k:=_to).
+        2: setoid_rewrite <- Heqy.
+        2: reflexivity.
+        erewrite insert_insert.
+        unfold xHMapInsert. simpl.
+        match goal with
+        | |- context [@addAdjustListPair _ _ _ ?a ?v _] => remember v
+        end.
+        enough (x0 = x).
+        destruct s0.
+        erewrite member_addAdjust; auto.
+        rewrite H3. auto.
+        subst x0.
+        destruct x, _value. simpl.
+        f_equal. lia.
+      + subst _from.
+        apply member_true_lookup in H1.
+        destruct H1.
+        setoid_rewrite H in Heqy.
+        discriminate.
+    Unshelve.
+    all: refine (BoolEq.pair_eqb_spec (X:=Z) (Y:=XUBInteger 256)).
+Qed.    
+
+
+Lemma transferFrom_from_not_member_balances: forall (_from :  address) (_to :  address) 
+                            (_value : uint256)
+                            (l: LedgerLRecord rec), 
+    let l0 := {$$ l with Ledger_LocalState := default $$} in
+    let l' := exec_state (Uinterpreter (@transferFrom rec def _ _ _ _ _from _to _value)) l0 in
+    let msg_sender := VMState_ι_msg_sender (l.(Ledger_VMState)) in
+    let balances0 := (_balances (l.(Ledger_MainState))) in    
+    let allowed0 := (_allowed (l.(Ledger_MainState))) in 
+    _from = _to -> 
+    keysDistinct balances0 ->
+    hmapIsMember (H7 := @pair_xbool_equable bool _ Z _ uint256 _  ) _from balances0  = false ->
+    _balances (l'.(Ledger_MainState)) =
+    if ((xIntGeb balances0 [_from]  _value : bool) && 
+        (xIntGeb allowed0 [_from] [msg_sender] _value : bool) ) then 
+         balances0 [_from] ← default
+    else balances0.
+Proof.
+    intros. transferFrom_start l l0 l'.
+    compute_rhs.    
+    compute in balances0, msg_sender, allowed0.
+
+    match goal with
+    | |- context [if ?b then false else true] => remember b
+    end.    
+    
+    case_eq b; intros; auto.
+    subst msg_sender.
+    subst _from.
+
+    apply member_false_lookup in H1.    
+
+    match goal with
+    | |- context [if ?b then _ else _] => remember b
+    end.    
+    
+    destruct b0.
+    -
+    erewrite lookup_some_find with (k:=_to).
+    erewrite lookup_none_find with (k:=_to).    
+    3: erewrite lookup_none_find with (k:=_to).    
+    3: unshelve erewrite lookup_addAdjust.    
+    3: refine (BoolEq.pair_eqb_spec (X:=Z) (Y:=XUBInteger 256)).
+    2, 3, 4: auto.
+    enough (_value = default).
+    subst _value.
+    simpl.
+    erewrite insert_insert.        
+    simpl.
+    match goal with
+    | |- context [@addAdjustListPair _ _ _ ?a ?v _] => remember v
+    end.
+    enough (x = default).
+    rewrite H. auto.
+    subst x.
+    simpl default.
+    f_equal.
+    remember ((uint2N _value <=?
+          uint2N (Common.hmapFindWithDefault (Build_XUBInteger 0) _to s0))%N).
+    setoid_rewrite <- Heqb1 in Heqb.
+    destruct b0.
+    + erewrite lookup_none_find with (k:=_to) in Heqb1.
+      destruct _value.
+      simpl in Heqb1 |- *.
+      symmetry in Heqb1.
+      apply N.leb_le in Heqb1.
+      unfold N.zero.
+      f_equal. lia.
+      auto.
+    + congruence.
+    -    
+    erewrite lookup_some_find with (k:=_to).
+    erewrite lookup_none_find with (k:=_to).    
+    3: erewrite lookup_none_find with (k:=_to).    
+    3: unshelve erewrite lookup_addAdjust.    
+    3: refine (BoolEq.pair_eqb_spec (X:=Z) (Y:=XUBInteger 256)).
+    2, 3, 4: auto.
+    enough (_value = default).
+    subst _value.
+    simpl.
+    erewrite insert_insert.        
+    simpl.
+    match goal with
+    | |- context [@addAdjustListPair _ _ _ ?a ?v _] => remember v
+    end.
+    enough (x = default).
+    rewrite H. auto.
+    subst x.
+    simpl default.
+    f_equal.
+    remember ((uint2N _value <=?
+          uint2N (Common.hmapFindWithDefault (Build_XUBInteger 0) _to s0))%N).
+    setoid_rewrite <- Heqb1 in Heqb.
+    destruct b0.
+    + erewrite lookup_none_find with (k:=_to) in Heqb1.
+      destruct _value.
+      simpl in Heqb1 |- *.
+      symmetry in Heqb1.
+      apply N.leb_le in Heqb1.
+      unfold N.zero.
+      f_equal. lia.
+      auto.
+    + congruence.
+  Unshelve.
+  all: refine (BoolEq.pair_eqb_spec (X:=Z) (Y:=XUBInteger 256)).
+Qed.  
+
+Lemma transferFrom_balances_keysDistinct: forall (_from :  address) (_to :  address) 
+                            (_value : uint256)
+                            (l: LedgerLRecord rec), 
+    let l0 := {$$ l with Ledger_LocalState := default $$} in
+    let l' := exec_state (Uinterpreter (@transferFrom rec def _ _ _ _ _from _to _value)) l0 in
+    let msg_sender := VMState_ι_msg_sender (l.(Ledger_VMState)) in
+    let balances0 := (_balances (l.(Ledger_MainState))) in
+    let balances := (_balances (l'.(Ledger_MainState))) in 
+    let allowed0 := (_allowed (l.(Ledger_MainState))) in     
+    keysDistinct balances0 ->  keysDistinct balances.
+Proof.
+    intros.
+    remember ((xIntGeb balances0 [_from]  _value : bool) && 
+              (xIntGeb allowed0 [_from] [msg_sender] _value : bool) ) as b1.
+    remember (eqb _from _to) as b2.
+    remember (hmapIsMember (H7 := @pair_xbool_equable bool _ Z _ uint256 _  ) _from balances0) as b3.
+    subst balances. subst l'. subst l0. subst balances0. subst allowed0. subst msg_sender.
+    destruct b1, b2, b3. 
+    -   rewrite transferFrom_from_member_balances; auto.  
+        apply BoolEq.eqb_spec_intro. auto.
+    -   rewrite transferFrom_from_not_member_balances; auto.
+        setoid_rewrite <- Heqb1.
+        apply insert_kd. assumption.
+        apply BoolEq.eqb_spec_intro. auto.
+    -   rewrite transferFrom_others_balances; auto.
+        rewrite <- Heqb1.
+        repeat apply insert_kd. assumption.
+        unfold not; intros. apply BoolEq.eqb_spec_intro in H0.
+        rewrite H0 in Heqb2. discriminate.
+    -   rewrite transferFrom_others_balances; auto.
+        rewrite <- Heqb1.
+        repeat apply insert_kd. assumption.
+        unfold not; intros. apply BoolEq.eqb_spec_intro in H0.
+        rewrite H0 in Heqb2. discriminate.
+    -   rewrite transferFrom_from_member_balances; auto.
+        apply BoolEq.eqb_spec_intro. auto.
+    -   rewrite transferFrom_from_not_member_balances; auto.
+        rewrite <- Heqb1. assumption.
+        apply BoolEq.eqb_spec_intro. auto.
+    -   rewrite transferFrom_others_balances; auto.
+        rewrite <- Heqb1. assumption.
+        unfold not; intros. apply BoolEq.eqb_spec_intro in H0.
+        rewrite H0 in Heqb2. discriminate.
+    -   rewrite transferFrom_others_balances; auto.
+        rewrite <- Heqb1. assumption.
+        unfold not; intros. apply BoolEq.eqb_spec_intro in H0.
+        rewrite H0 in Heqb2. discriminate.
+Qed.
+
+Lemma transferFrom_balances_sum: forall (_from :  address) (_to :  address) 
+                            (_value : uint256)
+                            (l: LedgerLRecord rec), 
+    let l0 := {$$ l with Ledger_LocalState := default $$} in
+    let l' := exec_state (Uinterpreter (@transferFrom rec def _ _ _ _ _from _to _value)) l0 in
+    let msg_sender := VMState_ι_msg_sender (l.(Ledger_VMState)) in
+    let balances0 := (_balances (l.(Ledger_MainState))) in
+    let balances := (_balances (l'.(Ledger_MainState))) in
+    let allowed0 := (_allowed (l.(Ledger_MainState))) in  
+    keysDistinct balances0 ->    
+    hmapBSum balances = hmapBSum balances0.
+Proof.
+    intros.
+    remember ((xIntGeb balances0 [_from]  _value : bool) && 
+              (xIntGeb allowed0 [_from] [msg_sender] _value : bool) ) as b1.
+    remember (eqb _from _to) as b2.
+    remember (hmapIsMember (H7 := @pair_xbool_equable bool _ Z _ uint256 _  ) _from balances0) as b3.
+    subst balances. subst l'. subst l0. subst balances0. subst allowed0. subst msg_sender.
+    destruct b1, b2, b3.   
+    - (* 1/8 *) rewrite transferFrom_from_member_balances; auto.
+      apply BoolEq.eqb_spec_intro. auto.
+    - (* 2/8 *) rewrite transferFrom_from_not_member_balances; auto.
+      setoid_rewrite <- Heqb1.
+      unfold hmapBSum.
+      rewrite mapBN2N_addAdjust.
+      rewrite hmapSumAdjust.
+      rewrite lookup_none_find.
+      simpl. f_equal. unfold N.zero. lia. 
+      symmetry in Heqb3.
+      apply member_false_lookup in Heqb3. 
+      rewrite mapBN2N_hmapLookup2.
+      setoid_rewrite Heqb3. auto.
+      1,4: refine pair_xbool_equable.    
+      1,3: refine BoolEq.pair_eqb_spec.
+      2: assumption.
+      apply mapBN2N_keysDistinct. assumption.
+      apply BoolEq.eqb_spec_intro.
+      auto.
+    - (* 3/8 *) rewrite transferFrom_others_balances; auto.
+       rewrite <- Heqb1.
+       unfold hmapBSum.
+       repeat rewrite mapBN2N_addAdjust.
+       repeat rewrite hmapSumAdjust.
+       remember (hmapSum (mapBN2N (_balances (Ledger_MainState l)))).
+       (* setoid_rewrite <- Heqn. *)
+       remember ((mapBN2N (_balances (Ledger_MainState l))) [_to]?).
+       destruct y.
+       + erewrite 2lookup_some_find with (k:=_to).
+         2: setoid_rewrite <- Heqy.
+         2: reflexivity.                  
+         rewrite mapBN2N_hmapLookup2 in Heqy.
+         all: cycle 3.
+         enough ((_balances (Ledger_MainState l)) [_to] ? = Some (Build_XUBInteger n0)).
+         setoid_rewrite H0. reflexivity.
+         rewrite mapBN2N_hmapLookup2 in Heqy.
+         remember ((_balances (Ledger_MainState l)) [_to] ?).
+         setoid_rewrite <- Heqy0 in Heqy.         
+         destruct y. simpl in Heqy. inversion Heqy.
+         destruct x.  auto. inversion Heqy.
+         all: cycle 2.
+         symmetry in Heqb3.
+         apply member_true_lookup in Heqb3.
+         destruct Heqb3.
+         erewrite lookup_some_find with (k:=_from).
+         2: setoid_rewrite H0.
+         2: reflexivity.         
+         erewrite lookup_some_find with (k:=_from).
+         2: erewrite lookup_addAdjust_another.
+         2: rewrite mapBN2N_hmapLookup2.
+         2: setoid_rewrite H0.
+         2: reflexivity.
+         destruct x, _value.
+         simpl. 
+         f_equal.
+         enough(n1 >= n2). lia.
+         symmetry in Heqb1.
+         apply andb_prop in Heqb1. inversion Heqb1.
+         eapply lookup_some_find in H0.
+         erewrite H0 in H1. simpl in H1.
+         apply N.leb_le in H1.
+         lia.
+         1,4,6: refine pair_xbool_equable.    
+         1,3,4: refine BoolEq.pair_eqb_spec.
+         unfold not; intros. apply BoolEq.eqb_spec_intro in H1.
+         rewrite H1 in Heqb2. discriminate.
+      + erewrite 2lookup_none_find with (k:=_to); auto.
+        2: rewrite mapBN2N_hmapLookup2 in Heqy.
+        2: remember ((_balances (Ledger_MainState l)) [_to] ?).
+        2: setoid_rewrite <- Heqy0. 
+        2: setoid_rewrite <- Heqy0 in Heqy.
+        2: destruct y; auto.
+        2: discriminate.           
+        rewrite mapBN2N_hmapLookup2 in Heqy.
+        remember ((_balances (Ledger_MainState l)) [_to] ?).
+        setoid_rewrite <- Heqy0 in Heqy.
+        destruct y. discriminate.
+        remember ((_balances (Ledger_MainState l)) [_from]?).
+        destruct y.
+          *
+          erewrite 2lookup_some_find with (k:=_from).      
+          3: setoid_rewrite <- Heqy1.
+          3: reflexivity.
+          2: erewrite lookup_addAdjust_another.
+          2: rewrite mapBN2N_hmapLookup2.
+          2: setoid_rewrite <- Heqy1.
+          2: reflexivity.
+          destruct x, _value. simpl. unfold N.zero.
+          f_equal. enough (n0 >= n1). lia.
+          symmetry in Heqb1.
+          apply andb_prop in Heqb1. inversion Heqb1.
+          erewrite lookup_some_find in H0.
+          2: setoid_rewrite <- Heqy1.
+          2: reflexivity.
+          simpl in H0.        
+          apply N.leb_le in H0.
+          lia.
+          refine pair_xbool_equable.
+          refine BoolEq.pair_eqb_spec.
+          unfold not; intros. apply BoolEq.eqb_spec_intro in H0.
+          rewrite H0 in Heqb2. discriminate.
+          * symmetry in Heqb3.
+            apply member_true_lookup in Heqb3.
+            destruct Heqb3.
+            setoid_rewrite H0 in Heqy1. 
+            discriminate.
+          * refine pair_xbool_equable.
+          * refine BoolEq.pair_eqb_spec.
+          * refine pair_xbool_equable.
+          * refine BoolEq.pair_eqb_spec.
+      + apply mapBN2N_keysDistinct. assumption.
+      + apply insert_kd. apply mapBN2N_keysDistinct. assumption.
+      + refine pair_xbool_equable.
+      + refine BoolEq.pair_eqb_spec.
+      + assumption.
+      + refine pair_xbool_equable.
+      + refine BoolEq.pair_eqb_spec.
+      + apply insert_kd.  assumption.
+      + unfold not; intros. apply BoolEq.eqb_spec_intro in H0.
+        rewrite H0 in Heqb2. discriminate.
+    - (* 4/8 *) rewrite transferFrom_others_balances; auto.
+       rewrite <- Heqb1.
+       unfold hmapBSum.
+       repeat rewrite mapBN2N_addAdjust.
+       repeat rewrite hmapSumAdjust.
+       remember (hmapSum (mapBN2N (_balances (Ledger_MainState l)))).
+       (* setoid_rewrite <- Heqn. *)
+       remember ((mapBN2N (_balances (Ledger_MainState l))) [_to]?).
+       destruct y.
+       + erewrite 2lookup_some_find with (k:=_to).
+         2: setoid_rewrite <- Heqy.
+         2: reflexivity.                  
+         rewrite mapBN2N_hmapLookup2 in Heqy.
+         all: cycle 3.
+         enough ((_balances (Ledger_MainState l)) [_to] ? = Some (Build_XUBInteger n0)).
+         setoid_rewrite H0. reflexivity.
+         rewrite mapBN2N_hmapLookup2 in Heqy.
+         remember ((_balances (Ledger_MainState l)) [_to] ?).
+         setoid_rewrite <- Heqy0 in Heqy.         
+         destruct y. simpl in Heqy. inversion Heqy.
+         destruct x.  auto. inversion Heqy.
+         all: cycle 2.
+         symmetry in Heqb3.
+         apply member_false_lookup in Heqb3.         
+         erewrite lookup_none_find with (k:=_from).
+         2: setoid_rewrite Heqb3.
+         2: reflexivity.         
+         erewrite lookup_none_find with (k:=_from).
+         2: erewrite lookup_addAdjust_another.
+         2: rewrite mapBN2N_hmapLookup2.
+         2: setoid_rewrite Heqb3.
+         2: reflexivity.
+         destruct  _value.
+         simpl. 
+         f_equal. unfold N.zero.
+         enough (n1 = 0). rewrite H0. lia.
+         symmetry in Heqb1.
+         apply andb_prop in Heqb1. inversion Heqb1.
+         erewrite lookup_none_find in H0. simpl in H0.         
+         apply N.leb_le in H0. unfold N.zero in H0.
+         lia. auto.
+         1,4,6: refine pair_xbool_equable.    
+         1,3,4: refine BoolEq.pair_eqb_spec.
+         unfold not; intros. apply BoolEq.eqb_spec_intro in H0.
+         rewrite H0 in Heqb2. discriminate.
+      + erewrite 2lookup_none_find with (k:=_to); auto.
+        2: rewrite mapBN2N_hmapLookup2 in Heqy.
+        2: remember ((_balances (Ledger_MainState l)) [_to] ?).
+        2: setoid_rewrite <- Heqy0. 
+        2: setoid_rewrite <- Heqy0 in Heqy.
+        2: destruct y; auto.
+        2: discriminate.           
+        rewrite mapBN2N_hmapLookup2 in Heqy.
+        remember ((_balances (Ledger_MainState l)) [_to] ?).
+        setoid_rewrite <- Heqy0 in Heqy.
+        destruct y. discriminate.
+        remember ((_balances (Ledger_MainState l)) [_from]?).
+        destruct y.
+        * symmetry in Heqb3.
+          rewrite member_false_lookup in Heqb3.
+          setoid_rewrite Heqb3 in Heqy1.
+          discriminate.
+        * erewrite 2lookup_none_find with (k:=_from).
+        3: setoid_rewrite <- Heqy1.
+        3: reflexivity.
+        2: erewrite lookup_addAdjust_another.
+        2: rewrite mapBN2N_hmapLookup2.
+        2: setoid_rewrite <- Heqy1.
+        2: reflexivity.
+        enough (_value = default). rewrite H0.
+        simpl. unfold N.zero.
+        f_equal. lia.         
+        symmetry in Heqb1.
+        apply andb_prop in Heqb1. inversion Heqb1.
+        erewrite lookup_none_find in H0.
+        destruct _value.
+        simpl in H0. unfold N.zero in H0.
+        apply N.leb_le in H0. simpl default.
+        f_equal. unfold N.zero. lia.
+        auto.
+        refine pair_xbool_equable.
+        refine BoolEq.pair_eqb_spec.
+        unfold not; intros. apply BoolEq.eqb_spec_intro in H0.
+        rewrite H0 in Heqb2. discriminate.
+        * refine pair_xbool_equable.
+        * refine BoolEq.pair_eqb_spec.
+        * refine pair_xbool_equable.
+        * refine BoolEq.pair_eqb_spec.
+        + apply mapBN2N_keysDistinct. assumption.
+        + apply insert_kd. apply mapBN2N_keysDistinct. assumption.
+        + refine pair_xbool_equable.
+        + refine BoolEq.pair_eqb_spec.
+        + assumption.
+        + refine pair_xbool_equable.
+        + refine BoolEq.pair_eqb_spec.
+        + apply insert_kd.  assumption.
+        + unfold not; intros. apply BoolEq.eqb_spec_intro in H0.
+        rewrite H0 in Heqb2. discriminate.    
+      - (* 5/8 *) rewrite transferFrom_from_member_balances; auto.
+        apply BoolEq.eqb_spec_intro. auto.
+      - (* 6/8 *) rewrite transferFrom_from_not_member_balances; auto.
+        rewrite <- Heqb1. auto.
+        apply BoolEq.eqb_spec_intro. auto.
+      - (* 7/8 *) rewrite transferFrom_others_balances; auto.
+        rewrite <- Heqb1. auto.
+        unfold not; intros. apply BoolEq.eqb_spec_intro in H0.
+        rewrite H0 in Heqb2. discriminate.
+      - (* 8/8 *) rewrite transferFrom_others_balances; auto.
+        rewrite <- Heqb1. auto.
+        unfold not; intros. apply BoolEq.eqb_spec_intro in H0.
+        rewrite H0 in Heqb2. discriminate.
+Qed.   
